---
title: Test-0114
author: Wang
date: 2024-01-14
category: Jekyll
layout: post
mermaid: true
---


$$\begin{aligned}
& K_s-K_n=2 \sum_{|k|<k_F} \varepsilon_k\left(h_k-1\right)+2 \sum_{|k|>k_F} \varepsilon_k h_k \\
& =2 \sum_{|k|<k_F}\left|\varepsilon_k\right|\left(1-h_k\right)+2 \sum_{|k|>k_F} \varepsilon_k h_k=4 \sum_{|k| k_F} \varepsilon_k h_k
\end{aligned}$$
 这里考虑到了 $1-h_k(-\varepsilon)=h_k(\varepsilon)$

![original image](https://cdn.mathpix.com/snip/images/Zk83NkUPFMumptGaSHkqRx6CZl_g53IK6cfmeaExzX4.original.fullsize.png)

一直推，得到

\begin{aligned}
& K_s-K_n=4 \sum_{\mid k>k_F} \varepsilon_k h_k=2 \sum_{|k| k_F} \varepsilon_k\left[1-\frac{\varepsilon_k}{\sqrt{\left|\varepsilon_k\right|^2+\Delta^2}}\right] \\
& =2 N(0) \int_0^{\hbar \omega_D}\left[\varepsilon-\frac{\varepsilon^2}{\sqrt{\varepsilon^2+\Delta^2}}\right] d \varepsilon=\frac{\Delta^2}{V}-\frac{1}{2} N(0) \Delta^2
\end{aligned}
